examples/cannon/CannonIAproof.v
@@ -9,39 +9,39 @@ Module CannonIA. Section CannonIA.
   Import CannonAS.
   Context `{!invG α Σ Γ, !subG Γ Σ, !sinvG Σ Γ α β τ, !CannonAGΓ Γ}.
 
+  Context (u_s : univ_id).
+  Context (Spc_s : string → option fspec).
+
   Definition Ist : nat → alist key Any.t → alist key Any.t → iProp Σ :=
     (λ _ st_s st_t,
-      (⌜st_s = [(CannonA.v_lv, 1%Z↑)] /\ st_t = [(CannonI.v_lv, 1%Z↑)]⌝ ∗
-      (Ready ∨ Fired))
+      (⌜st_s = [(CannonA.v_lv, 1%Z↑)] /\ st_t = [(CannonI.v_lv, 1%Z↑)]⌝ ∗ Ready)
+      ∨ Fired
     )%I.
-
-  Variable u: univ_id.
-  Variable SpcCannon : string -> option fspec.
   
-  Local Definition CannonAMod := (CannonA.t u SpcCannon).
+  Local Definition CannonAMod := (CannonA.t u_s Spc_s).
   Local Definition CannonIMod := (CannonI.t).
 
   Lemma simF_fire : HSim.sim_fun open CannonAMod CannonIMod Ist CannonName.fire.
   Proof.
-    init_simF.
+    winit_simF u_s 0.
 
-    steps_l. iDestruct "ASM" as "((%Y & B) & %Q)". subst. hss.
-    unfold Ist. iDestruct "IST" as "[[% %] [R | F]]"; cycle 1. 
+    wsteps_l. iDestruct "ASM" as "((%Y & B) & %Q)". subst. hss.
+    unfold Ist. iDestruct "IST" as "[[% R] | F]"; des; subst; cycle 1. 
     (* already fired *)
     { iExFalso. iApply FiredBall. iFrame. }
 
-    steps_r. force_r. iSplitR.
-    { iPureIntro. rewrite Any.upcast_downcast. et. }
-    steps_r. change (1 `div` 1)%Z with 1%Z.
-    step. steps_l. force_l. force_l. instantiate (1:=(1%Z)↑). iSplitR; et.
-    steps_r. ss.
+    wsteps_r. hss. wsteps_r.
+    change (1 `div` 1)%Z with 1%Z. wstep. wsteps_r.
+    rewrite /alist_upd /_alist_upd /=. replace (1 - 1)%Z with 0%Z by nia.
+    wsteps_l. wforces_l. iSplitR; eauto. wstep.
+    iSplit; eauto. iRight. iApply ReadyBall; iFrame.
   Qed.
 
   Theorem sim : HSim.t open CannonAMod CannonIMod CannonA.init_cond Ist.
   Proof.
     init_sim.
-    - iIntros "IC". unfold Ist, CannonA.init_cond. iSplitR; et.
-    - eapply simF_fire; eauto.
+    - iIntros "IC". unfold Ist, CannonA.init_cond. iLeft. iFrame; eauto.
+    - eapply simF_fire.
   Qed.
 
   Theorem correct :
@@ -49,7 +49,6 @@ Module CannonIA. Section CannonIA.
       (CannonAMod, CannonA.init_cond)
       (CannonIMod, emp%I).
   Proof.
-    eapply main_adequacy.
-    apply sim.
+    eapply main_adequacy, sim.
   Qed.
 End CannonIA. End CannonIA.
